src/Utils/UnionFind.v
@@ -10,7 +10,13 @@
    URL: https://www.lri.fr/~filliatr/ftp/publis/puf-wml07.pdf.
 *)
 
+Require ZArith.
+
+From Tries Require Import Canonical.
+
 From Utils Require Import Utils Natlike ArrayList.
+From Utils Require TrieMap NatlikePos.
+
 
 
 
@@ -20,9 +26,9 @@ From Utils Require Import Utils Natlike ArrayList.
 Section UnionFind.
   
   Context {idx : Type}
-          `{Natlike idx}
-          {array : Type -> Type}
-          `{ArrayList idx array}.
+    `{Natlike_ok idx}
+    {array : Type -> Type}
+    `{ArrayList idx array}.
 
   Notation zero := (zero : idx).
 
@@ -65,6 +71,7 @@ Section UnionFind.
         (f,r)
       ).
 
+  
   Definition find '(MkUF ra pa mr) x :=
     let (f,cx) := find_aux mr pa x in
     (MkUF ra f mr, cx).
@@ -89,11 +96,9 @@ Section UnionFind.
            else
              (MkUF (set ra cx (succ rx))
                   (set pa cy cx)
-                       (max mr (succ rx)), cx).
+                  (max mr (succ rx)), cx).
+    
 End UnionFind.
-
-(*TODO*)
-Class UnionFind_ok := {}.
 
 
 (* All definitions and proofs need to be generic over arraylist implementations.
@@ -113,9 +118,10 @@ Module Int63UnionFind.
   Axiom TODO : forall A, A.
   
   #[refine] Instance int63eqb : Eqb int := { eqb := Int63Natlike.eqb}.
-  exact Int63Natlike.eqb_eq.
-  apply TODO.  apply TODO.
-  exact Int63Natlike.eq_dec.
+  - exact Int63Natlike.eqb_eq.
+  - apply TODO.
+  - apply TODO.
+  - exact Int63Natlike.eq_dec.
   Defined.
 
   Instance natlike_int63 : Natlike int :=
@@ -152,3 +158,331 @@ Module Int63UnionFind.
 
 End Int63UnionFind.
   
+Module PositiveUnionFind.
+  Import ZArith.
+  Import TrieMap.TrieArrayList.
+  Open Scope positive.
+
+  Notation union_find := (@UnionFind.union_find positive trie_array).
+
+  
+  Definition is_parent '(MkUF ra pa mr : union_find) x y : Prop :=
+    get pa y = x.
+
+  (* TODO: will there be issues w/ positive overflowing here?
+     TODO: if we assume is_top = false, do the issues go away?
+   *)
+  Inductive parent_degree (pa : trie_array positive) : positive -> positive -> Prop :=
+  | pdegree_0 i : get pa i = i -> parent_degree pa i 1
+  | pdegree_S i j n : get pa i = j -> parent_degree pa j n -> parent_degree pa i (succ n).
+  
+  Inductive parent_degree_bound (pa : trie_array positive) : positive -> positive -> Prop :=
+  | pdegree_b0_bound i n : get pa i = i -> parent_degree_bound pa i n
+  | pdegree_S_bound i j n m
+    : get pa i = j ->
+      parent_degree_bound pa j n ->
+      n < m ->
+      parent_degree_bound pa i m.
+  
+  Record trie_array_ok {A} (a : trie_array A) :=
+    {
+      len_gt_max_key : forall i e,
+        PTree.get i (snd (fst a)) = Some e ->
+        fst (fst a) > i
+    }.
+
+  Definition dense {A} (a : trie_array A) :=
+    forall i, i < fst (fst a) ->
+              if PTree.get i (snd (fst a)) then True else False.
+  
+  Record union_find_ok (u : union_find) :=
+    {
+      max_rank_ok : forall i, (get u.(rank) i) <= u.(max_rank);
+      ranks_ok : forall i, parent_degree_bound u.(parent) i (get u.(rank) i);
+      len_same : ArrayList.length u.(parent) = ArrayList.length u.(rank);
+      parents_ok : trie_array_ok u.(parent);
+      parents_dense : dense u.(parent);
+      rank_ok : trie_array_ok u.(rank);
+      rank_dense : dense u.(rank);
+    }.
+
+  (*TODO: move to Utils.v*)
+  Inductive equivalence_closure {A} (R : A -> A -> Prop) : A -> A -> Prop :=
+  | eq_clo_base a b : R a b -> equivalence_closure R a b
+  | eq_clo_refl a : equivalence_closure R a a
+  | eq_clo_trans a b c : equivalence_closure R a b -> equivalence_closure R b c -> equivalence_closure R a c
+  | eq_clo_sym a b : equivalence_closure R a b -> equivalence_closure R b a.
+
+  Hint Constructors equivalence_closure : utils.
+
+  Inductive parent_path (pa : trie_array positive) : positive -> positive -> Prop :=
+  | ppath_0 i : parent_path pa i i
+  | ppath_S i j k : get pa i = j -> parent_path pa j k -> parent_path pa i k.
+  Hint Constructors parent_path : utils.
+
+  Let uf_clo uf := equivalence_closure (is_parent uf).
+  
+  Lemma find_preserves_len_parents (uf : union_find) i uf' i'
+    : find uf i = (uf', i') ->
+      i < ArrayList.length uf.(parent) ->
+      ArrayList.length uf.(parent) =  ArrayList.length uf'.(parent).
+  Proof.    
+    destruct uf as [ra pa mr].
+    revert ra pa i uf' i'.
+    eapply Pos.peano_ind with (p:=mr);
+      intros;
+      destruct uf' as [ra' pa' mr'];
+      unfold trie_array in *; break; simpl in *.
+    {
+      revert H; case_match.
+      repeat (revert HeqH;case_match); simpl in *;
+        basic_goal_prep;
+          basic_utils_crush;
+        try congruence;
+        safe_invert H3;
+        rewrite Pos.max_l; Lia.lia.
+    }
+  Abort.
+
+  (*
+    
+  Lemma find_preserves_ok uf i uf' i'
+    : union_find_ok uf ->
+      find uf i = (uf', i') ->
+      (*TODO: do I want this condition?*)
+      i < ArrayList.length uf.(parent) ->
+      union_find_ok uf'.
+  Proof.
+    
+    destruct uf as [ra pa mr].
+    revert ra pa i uf' i'.
+    eapply Pos.peano_ind with (p:=mr);
+      intros; unfold trie_array in *; break.
+    {
+      destruct H;
+        revert H0; simpl in *.
+      case_match;
+      revert HeqH.
+      case_match;
+        revert HeqH.
+      {
+        case_match;
+          intro H'; symmetry in H'; apply Pos.eqb_eq in H'; subst;
+          intro H'; safe_invert H';
+          intro H'; safe_invert H';
+          constructor; eauto.
+      }
+      {
+        case_match.
+        {
+          intros _.
+          intro H'; safe_invert H';
+            intro H'; safe_invert H'.
+          assert (Pos.max p1 (i + 1) = p1).
+          {
+            eapply Pos.max_l.
+            destruct parents_ok0.
+            simpl in *.
+            symmetry in HeqH.
+            apply len_gt_max_key0 in HeqH.
+            Lia.lia.
+          }
+          {
+            constructor; simpl; eauto.
+            
+            simpl.
+      }
+        }
+        {
+          
+        }
+          
+    
+  Lemma find_preserves_relation uf i uf' i'
+    : union_find_ok uf ->
+      find uf i = (uf', i') ->
+      (forall x y, uf_clo uf x y <-> uf_clo uf' x y)
+      /\ (uf_clo uf i i').
+  Proof.
+    destruct uf as [ra pa mr].
+    revert ra pa i uf' i'.
+    eapply Pos.peano_ind with (p:=mr);
+      intros; unfold trie_array in *; break.
+    {
+      simpl in *.
+      revert H.
+      my_case Hir (PTree.get i r).
+      2:{
+      case_match.
+      revert HeqH.
+      case_match.
+    }
+  
+  (*TODO: not true because arrays are non-canonical due to default elt*)
+  Lemma get_set_same_existing (pa : trie_array positive) i
+    :  trie_array_ok pa ->
+       i < ArrayList.length pa -> set pa i (get pa i) = pa.
+  Proof.
+    destruct pa as [[? ?] ?]; simpl.
+    intros [?] iltp; simpl in *.
+    f_equal; f_equal.
+    {
+      unfold Pos.max.
+      destruct (Pos.compare_spec p (i+1)); try Lia.lia.
+    }
+    case_match.
+    2:{
+    [|f_equal].
+    cbn 
+    unfold get, set.
+    
+
+  Lemma find_aux_path pa mr
+    : forall i i' pa',
+      i < ArrayList.length pa ->
+        find_aux mr pa i = (pa', i') ->
+        parent_path pa i i'.
+  Proof.
+    cbn [find_aux Natlike.iter NatlikePos.natlike_positive].
+    revert pa.
+    
+    eapply Pos.peano_ind with (p:=mr);
+      intros; break.
+    {
+      cbn -[get set] in H0.
+      revert H0; case_match.
+      {        
+        basic_goal_prep;
+          basic_utils_crush.
+      }
+      {
+        destruct 
+      }
+    rewrite iter_succ in *; eauto.
+    2:{
+      apply is_top_spec; eauto.
+    }
+    revert H4; case_match.
+    { 
+      basic_goal_prep;
+        basic_utils_crush.
+    }
+    remember (iter _ _ _ _ _) as loop.
+    destruct loop.
+    basic_goal_prep;
+      basic_utils_crush.
+  Qed.
+
+  Lemma max_rank_upper_bound u
+    : union_find_ok u ->
+      forall i, parent_degree_bound u.(parent) i u.(max_rank).
+  Proof.
+    intro H'; destruct H'.
+    intro i.
+    specialize (ranks_ok0 i).
+    specialize (max_rank_ok0 i).
+    clear len_same0.
+    revert ranks_ok0 max_rank_ok0.
+    generalize (get (rank u) i).
+    induction 1.
+    {
+      constructor; eauto.
+    }
+    {
+      econstructor 2; eauto.
+      
+    }
+
+  Lemma find_aux_degree pa mr
+    : forall i i' pa',
+      find_aux mr pa i = (pa', i') ->
+      (get pa' i = i' /\
+      forall n j,
+      parent_degree_bound pa j n ->
+      parent_degree_bound pa' j n).
+  Proof.
+    revert pa.
+    unfold find_aux.
+    eapply natlike_ind with (n:=mr); auto;
+      [ rewrite iter_zero in * |];
+      basic_goal_prep;
+      basic_utils_crush.
+    rewrite iter_succ in *; eauto.
+    2:{
+      apply is_top_spec; eauto.
+    }
+    revert H4; case_match.
+    { 
+      basic_goal_prep;
+        basic_utils_crush.
+    }
+    remember (iter _ _ _ _ _) as loop.
+    destruct loop.
+    basic_goal_prep;
+      basic_utils_crush.
+    symmetry in Heqloop.
+    eapply H3 in Heqloop; eauto.
+    TODO: need to know about i, i'
+
+    Lemma decreasing_parent_degree_bound
+      : parent_degree_bound pa j n ->
+        parent_degree_bound (set pa i i') j n.
+                             
+
+    
+  Lemma find_aux_sound pa mr
+    : (forall i j, parent_degree pa i j -> leb j mr = true) ->
+      forall i i' pa',
+        find_aux mr pa i = (pa', i') ->
+        equivalence_closure (fun a b => get pa a = b) i i'.
+  Proof.
+    unfold find_aux.
+    revert pa.
+    eapply natlike_ind with (n:=mr); auto;
+      [ rewrite iter_zero in * |];
+      basic_goal_prep;
+      basic_utils_crush.
+    rewrite iter_succ in *; eauto.
+    2:{
+      apply is_top_spec; eauto.
+    }
+    {
+      revert H5; case_match.
+      { 
+        basic_goal_prep;
+          basic_utils_crush.
+      }
+      remember (iter _ _ _ _ _) as loop.
+      destruct loop.
+      basic_goal_prep;
+        basic_utils_crush.
+      eapply H3; eauto.
+      case_match'.
+      eapply eq_clo_trans.
+      rewrite iter_zero in H3.
+      
+      simpl in *.
+    }
+    auto.
+    
+    induction mr.
+ 
+  Lemma find_sound u i u' i'
+    : union_find_ok u -> find u i = (u', i') -> EqClo u i i'.
+  Proof.
+    destruct u.
+    unfold find.
+    unfold find_aux, union_find_ok.
+    simpl.
+    revert max_rank0 rank0 parent0.
+    eapply natlike_ind; eauto.
+    intros.
+      with (n:=max_rank0).
+
+    induction max_rank0.
+
+
+  TODO: generalize proofs to any unionfind
+*)
+
+End PositiveUnionFind.
